\documentclass{article} % required
\usepackage{amsmath}
\usepackage{amssymb}
\title{Quadratic Equations}
\author{James Blackburn}
\date{January 2022}
\begin{document}
\maketitle
\section{Proving the $\alpha$ $\beta$ formulas}
\begin{gather} 
\text{Define the quadratic equation with the variables } a, b, c\\
ax^2+bx+c = 0 \\
\text{Let } \alpha = x_1 \text{ (The first root of the equation)}\\
\alpha = \frac{-b + \sqrt{b^2-4ac}}{2a} \\
\text{Let } \beta = x_2 \text{ (The second root of the equation)}\\
\beta = \frac{-b - \sqrt{b^2-4ac}}{2a} \\
\text{Prove the formula } \alpha + \beta  = \frac{-b}{a} \text{ is true (via substitution)} \\ 
\begin{split}
 \frac{-b + \sqrt{b^2-4ac}}{2a} + \frac{-b - \sqrt{b^2-4ac}}{2a}\\ 
= \frac{-2b}{2a}\\ 
= \frac{-b}{a}
\end{split}
\\
\text{Prove the formula } \alpha\beta = \frac{c}{a}  \text{ is true (via substitution)} \\
\begin{split}
 \frac{-b + \sqrt{b^2-4ac}}{2a} \times \frac{-b - \sqrt{b^2-4ac}}{2a} \\
= \frac{(-b + \sqrt{b^2-4ac})(-b - \sqrt{b^2-4ac})}{4a^2} \\
= \frac{(-b)^2 - (\sqrt{b^2-4ac})^2}{4a^2}\\
= \frac{b^2 - (b^2-4ac)}{4a^2}\\
= \frac{4ac}{4a^2}\\
= \frac{c}{a}
\end{split}
\end{gather} 
\end{document}